infoflow: Move "EquivValid" out of "infoflow/", into "lib/".
More importantly, remove seL4 from the dependencies of "EquivValid", so
others can use it.

Also, we fixup the fallout.

lib/EquivValid.thy
@@ -8,10 +8,13 @@
  * @TAG(NICTA_GPL)
  *)
 
+(*
+ * A theoretical framework for reasoning about non-interference
+ * of monadic programs.
+ *)
+
 theory EquivValid
-imports
-  "../access-control/Syscall_AC"
-  (* doesn't really need this but its only dependants do *)
+imports Corres_UL
 begin
 
 section{* State equivalence validity *}
@@ -734,5 +737,254 @@ lemmas splits_spec_ev[wp_split] =
   spec_equiv_valid_guard_imp[OF bind_spec_ev] spec_equiv_valid_guard_imp[OF bindE_spec_ev]
   bind_spec_ev bindE_spec_ev
   spec_equiv_valid_guard_imp[OF if_spec_ev] if_spec_ev
+
+(* Miscellaneous rules. *)
+
+lemma assertE_ev[wp]:
+  "equiv_valid_inv I A \<top> (assertE b)"
+  unfolding assertE_def
+  apply wp
+  by simp
+
+lemma equiv_valid_2_bindE:
+  assumes g: "\<And>rv rv'. R' rv rv' \<Longrightarrow>
+      equiv_valid_2 D A A (E \<oplus> R) (Q rv) (Q' rv') (g rv) (g' rv')"
+  assumes h1: "\<lbrace>S\<rbrace> f \<lbrace>Q\<rbrace>,-"
+  assumes h2: "\<lbrace>S'\<rbrace> f' \<lbrace>Q'\<rbrace>,-"
+  assumes f: "equiv_valid_2 D A A (E \<oplus> R') P P' f f'"
+  shows "equiv_valid_2 D A A (E \<oplus> R) (P and S) (P' and S') (f >>=E g) (f' >>=E g')"
+  apply(unfold bindE_def)
+  apply(rule equiv_valid_2_guard_imp)
+    apply(rule_tac R'="E \<oplus> R'" and Q="case_sum \<top>\<top> Q" and Q'="case_sum \<top>\<top> Q'" and S=S and S'=S' in equiv_valid_2_bind)
+       apply(clarsimp simp: lift_def split: sum.splits)
+       apply(intro impI conjI allI)
+          apply(simp add: throwError_def)
+          apply(rule return_ev2)
+          apply simp
+         apply(simp)
+        apply(simp)
+       apply(fastforce intro: g)
+      apply(rule f)
+     apply(insert h1, fastforce simp: valid_def validE_R_def validE_def split: sum.splits)[1]
+    apply(insert h2, fastforce simp: valid_def validE_R_def validE_def split: sum.splits)[1]
+   by auto
+
+lemma rel_sum_comb_equals:
+  "((op =) \<oplus> (op =)) = (op =)"
+  apply(rule ext)
+  apply(rule ext)
+  apply(rename_tac a b)
+  apply(case_tac a, auto)
+  done
+
+definition spec_equiv_valid_2_inv where
+  "spec_equiv_valid_2_inv s I A R P P' f f' \<equiv> 
+      equiv_valid_2 I A A R (P and (op = s)) P' f f'"
+
+lemma spec_equiv_valid_def2:
+  "spec_equiv_valid s I A A P f =
+   spec_equiv_valid_2_inv s I A (op =) P P f f"
+  apply(simp add: spec_equiv_valid_def spec_equiv_valid_2_inv_def)
+  done
+
+lemma drop_spec_ev2_inv:
+  "equiv_valid_2 I A A R P P' f f' \<Longrightarrow> 
+   spec_equiv_valid_2_inv s I A R P P' f f'"
+  apply(simp add: spec_equiv_valid_2_inv_def)
+  apply(erule equiv_valid_2_guard_imp, auto)
+  done
+
+lemma spec_equiv_valid_2_inv_guard_imp:
+  "\<lbrakk>spec_equiv_valid_2_inv s I A R Q Q' f f'; \<And> s. P s \<Longrightarrow> Q s; \<And> s. P' s \<Longrightarrow> Q' s\<rbrakk> \<Longrightarrow>
+    spec_equiv_valid_2_inv s I A R P P' f f'"
+  by(auto simp: spec_equiv_valid_2_inv_def equiv_valid_2_def)
+
+lemma bind_spec_ev2:
+  assumes reads_res_2: "\<And> rv s' rv'. \<lbrakk>(rv, s') \<in> fst (f s); R' rv rv'\<rbrakk> \<Longrightarrow> spec_equiv_valid_2_inv s' I A R (Q rv) (Q' rv') (g rv) (g' rv')"
+  assumes reads_res_1: "spec_equiv_valid_2_inv s I A R' P P' f f'"
+  assumes hoare: "\<lbrace>S\<rbrace> f \<lbrace>Q\<rbrace>"
+  assumes hoare': "\<lbrace>S'\<rbrace> f' \<lbrace>Q'\<rbrace>"
+  shows "spec_equiv_valid_2_inv s I A R (P and S) (P' and S') (f >>= g) (f' >>= g')"
+  using reads_res_1
+  apply (clarsimp simp: spec_equiv_valid_2_inv_def equiv_valid_2_def bind_def split_def)
+  apply (erule_tac x=t in allE)
+  apply clarsimp
+  apply (drule_tac x="(a, b)" in bspec, assumption)
+  apply (drule_tac x="(ab, bb)" in bspec, assumption)
+  apply clarsimp
+  apply (cut_tac rv="a" and s'="b" in reads_res_2)
+    apply assumption
+   apply assumption
+  apply (clarsimp simp: spec_equiv_valid_2_inv_def equiv_valid_2_def)
+  apply(drule_tac x=bb in spec)
+  apply clarsimp
+  using hoare hoare'
+  apply (fastforce simp: valid_def)+
+  done
+
+lemma spec_equiv_valid_2_inv_bindE:
+  assumes g: "\<And>rv s' rv'. \<lbrakk>(Inr rv, s') \<in> fst (f s); R' rv rv'\<rbrakk> \<Longrightarrow>
+      spec_equiv_valid_2_inv s' I A (E \<oplus> R) (Q rv) (Q' rv') (g rv) (g' rv')"
+  assumes h1: "\<lbrace>S\<rbrace> f \<lbrace>Q\<rbrace>,-"
+  assumes h2: "\<lbrace>S'\<rbrace> f' \<lbrace>Q'\<rbrace>,-"
+  assumes f: "spec_equiv_valid_2_inv s I A (E \<oplus> R') P P' f f'"
+  shows "spec_equiv_valid_2_inv s I A (E \<oplus> R) (P and S) (P' and S') (f >>=E g) (f' >>=E g')"
+  apply(unfold bindE_def)
+  apply(rule spec_equiv_valid_2_inv_guard_imp)
+    apply(rule_tac R'="E \<oplus> R'" and Q="case_sum \<top>\<top> Q" and Q'="case_sum \<top>\<top> Q'" and S=S and S'=S' in bind_spec_ev2)
+       apply(clarsimp simp: lift_def split: sum.splits)
+       apply(intro impI conjI allI)
+          apply(simp add: throwError_def)
+          apply(rule drop_spec_ev2_inv[OF return_ev2])
+          apply simp
+         apply(simp)
+        apply(simp)
+       apply(fastforce intro: g)
+      apply(rule f)
+     apply(insert h1, fastforce simp: valid_def validE_R_def validE_def split: sum.splits)[1]
+    apply(insert h2, fastforce simp: valid_def validE_R_def validE_def split: sum.splits)[1]
+   by auto
+
+lemma trancl_subset_equivalence:
+  "\<lbrakk>(a, b) \<in> r'\<^sup>+; \<forall>x. (a, x)\<in>r'\<^sup>+ \<longrightarrow> Q x; \<forall>x y. Q x \<longrightarrow> ((y, x) \<in> r) = ((y, x) \<in> r')\<rbrakk> \<Longrightarrow> (a, b) \<in> r\<^sup>+"
+  apply(induct a b rule: trancl.induct)
+   apply(blast)
+  apply(simp)
+  apply(rule_tac b=b in trancl_into_trancl)
+   apply(simp)
+  apply(erule_tac x=c in allE)
+  apply(subgoal_tac "(a, c) \<in> r'\<^sup>+")
+   apply(auto)
+   done
+
+lemma equiv_valid_rv_gets_compD:
+  "equiv_valid_rv_inv I A R P (gets (f \<circ> g)) \<Longrightarrow>
+   equiv_valid_rv_inv I A (\<lambda> rv rv'. R (f rv) (f rv')) P (gets g)"
+  apply(clarsimp simp: equiv_valid_2_def gets_def bind_def return_def get_def)
+  done
+
+
+lemma liftE_ev2:
+  "equiv_valid_2 I A B R P P' f f' \<Longrightarrow>
+   equiv_valid_2 I A B (E \<oplus> R) P P' (liftE f) (liftE f')"
+  apply(clarsimp simp: liftE_def equiv_valid_2_def bind_def return_def)
+  apply fastforce
+  done
+
+lemma whenE_spec_ev2_inv:
+  assumes a: "b \<Longrightarrow> spec_equiv_valid_2_inv s I A R P P' m m'"
+  assumes r: "\<And> x. R x x"
+  shows "spec_equiv_valid_2_inv s I A R P P' (whenE b m) (whenE b m')"
+  unfolding whenE_def 
+  apply (auto intro: a simp: returnOk_def intro!: drop_spec_ev2_inv[OF return_ev2] intro: r)
+  done
+
+lemma whenE_spec_ev:
+  assumes a: "b \<Longrightarrow> spec_equiv_valid_inv s I A P m"
+  shows "spec_equiv_valid_inv s I A P  (whenE b m) "
+  unfolding whenE_def 
+  apply (auto intro: a simp: returnOk_def intro!: drop_spec_ev[OF return_ev_pre])
+  done
+
+
+lemma spec_equiv_valid_2_inv_by_spec_equiv_valid:
+  "\<lbrakk>spec_equiv_valid s I A A P f; P' = P; f' = f;
+    (\<And> a. R a a)\<rbrakk> \<Longrightarrow>
+       spec_equiv_valid_2_inv s I A R P P' f f'"
+  apply(clarsimp simp: spec_equiv_valid_def spec_equiv_valid_2_inv_def)
+  apply(fastforce simp: equiv_valid_2_def)
+  done
+
+lemma mapM_ev'':
+  assumes reads_res: "\<And> x. x \<in> set lst \<Longrightarrow> equiv_valid_inv D A (P x) (m x)"
+  assumes inv: "\<And> x. x \<in> set lst \<Longrightarrow> \<lbrace> \<lambda>s. \<forall>x\<in>set lst. P x s \<rbrace> m x \<lbrace> \<lambda>_ s. \<forall>x\<in>set lst. P x s \<rbrace>"
+  shows "equiv_valid_inv D A (\<lambda> s. \<forall>x\<in>set lst. P x s) (mapM m lst)"
+  apply(rule mapM_ev)
+  apply(rule equiv_valid_guard_imp[OF reads_res], simp+)
+  apply(wp inv, simp)
+  done
+
+lemma mapM_x_ev'':
+  assumes reads_res: "\<And> x. x \<in> set lst \<Longrightarrow> equiv_valid_inv D A (P x) (m x)"
+  assumes inv: "\<And> x. x \<in> set lst \<Longrightarrow> \<lbrace> \<lambda>s. \<forall>x\<in>set lst. P x s \<rbrace> m x \<lbrace> \<lambda>_ s. \<forall>x\<in>set lst. P x s \<rbrace>"
+  shows "equiv_valid_inv D A (\<lambda> s. \<forall>x\<in>set lst. P x s) (mapM_x m lst)"
+  apply(rule mapM_x_ev)
+  apply(rule equiv_valid_guard_imp[OF reads_res], simp+)
+  apply(wp inv, simp)
+  done
+
+lemma catch_ev[wp]:
+  assumes ok:
+    "equiv_valid I A A P f"
+  assumes err:
+    "\<And> e. equiv_valid I A A (E e) (handler e)" 
+  assumes hoare:
+    "\<lbrace> P \<rbrace> f -, \<lbrace> E \<rbrace>"
+  shows
+  "equiv_valid I A A P (f <catch> handler)"
+  apply(simp add: catch_def)
+  apply (wp err ok | wpc | simp)+
+   apply(insert hoare[simplified validE_E_def validE_def])[1]
+   apply(simp split: sum.splits)
+  by simp
+
+lemma equiv_valid_rv_trivial:
+  assumes inv: "\<And> P. \<lbrace> P \<rbrace> f \<lbrace> \<lambda>_. P \<rbrace>"
+  shows "equiv_valid_rv_inv I A \<top>\<top> \<top> f"
+  by(auto simp: equiv_valid_2_def dest: state_unchanged[OF inv])
+
+lemma equiv_valid_2_trivial:
+  assumes inv: "\<And> P. \<lbrace> P \<rbrace> f \<lbrace> \<lambda>_. P \<rbrace>"
+  assumes inv': "\<And> P. \<lbrace> P \<rbrace> f' \<lbrace> \<lambda>_. P \<rbrace>"
+  shows "equiv_valid_2 I A A \<top>\<top> \<top> \<top> f f'"
+  by(auto simp: equiv_valid_2_def dest: state_unchanged[OF inv] state_unchanged[OF inv'])
+
+lemma gen_asm_ev2_r:
+  "\<lbrakk>P' \<Longrightarrow> equiv_valid_2 I A B R P Q f f'\<rbrakk> \<Longrightarrow>
+   equiv_valid_2 I A B R P  (Q and (K P')) f f'"
+  apply(fastforce simp: equiv_valid_2_def)
+  done
+
+lemma gen_asm_ev2_l:
+  "\<lbrakk>P \<Longrightarrow> equiv_valid_2 I A B R Q P' f f'\<rbrakk> \<Longrightarrow>
+   equiv_valid_2 I A B R (Q and (K P)) P' f f'"
+  apply(fastforce simp: equiv_valid_2_def)
+  done
+
+lemma gen_asm_ev2_r':
+  "\<lbrakk>P' \<Longrightarrow> equiv_valid_2 I A B R P \<top> f f'\<rbrakk> \<Longrightarrow>
+   equiv_valid_2 I A B R P (\<lambda>s. P') f f'"
+  apply(fastforce simp: equiv_valid_2_def)
+  done
+
+lemma gen_asm_ev2_l':
+  "\<lbrakk>P \<Longrightarrow> equiv_valid_2 I A B R \<top> P' f f'\<rbrakk> \<Longrightarrow>
+   equiv_valid_2 I A B R (\<lambda>s. P) P' f f'"
+  apply(fastforce simp: equiv_valid_2_def)
+  done
+
+lemma equiv_valid_rv_liftE_bindE:
+  assumes ev1:
+  "equiv_valid_rv_inv I A W P f"
+  assumes ev2:
+  "\<And> rv rv'. W rv rv' \<Longrightarrow> equiv_valid_2 I A A R (Q rv) (Q rv') (g rv) (g rv')"
+  assumes hoare:
+  "\<lbrace> P \<rbrace> f \<lbrace> Q \<rbrace>"
+  shows "equiv_valid_rv_inv I A R P ((liftE f) >>=E g)"
+  apply(unfold bindE_def)
+  apply(rule_tac Q="\<lambda> rv. K (\<forall> v. rv \<noteq> Inl v) and (\<lambda> s. \<forall> v. rv = Inr v \<longrightarrow> Q v s)" in equiv_valid_rv_bind)
+    apply(rule_tac E="dc" in equiv_valid_2_liftE)
+    apply(rule ev1)
+   apply(clarsimp simp: lift_def split: sum.split)
+   apply(insert ev2, fastforce simp: equiv_valid_2_def)[1]
+  apply(insert hoare, clarsimp simp: valid_def liftE_def bind_def return_def split_def)
+  done
+
+lemma if_evrv:
+  assumes "b \<Longrightarrow> equiv_valid_rv_inv I A R P f"
+  assumes "\<not> b \<Longrightarrow> equiv_valid_rv_inv I A R Q g"
+  shows "equiv_valid_rv_inv I A R (\<lambda>s. (b \<longrightarrow> P s) \<and> (\<not>b \<longrightarrow> Q s)) (if b then f else g)"
+  apply (clarsimp split: split_if)
+  using assms by blast
 
 end
